core/properties/universality/Universality.v
@@ -44,6 +44,7 @@ Proof.
   unfold EvalUserExpressions.evalOutputPatternLink.
   unfold instantiateTrOnModel.
   unfold instantiateTrOnPiece.
+  unfold traceTrOnModel.
   unfold traceTrOnPiece.
   unfold traceRuleOnPiece.
   unfold traceIterationOnPiece.
